Order/Cleaning -- Adding and restructuring sections

src/IsoCan.v
@@ -60,6 +60,10 @@ Section IsoCan.
     (* add conditions on the input *)
     Variable hashTerm : term I B L -> h.
     Hypothesis perfectHashingSchemeTerm : injective hashTerm.
+    Variable hashTuple : seq h -> h.
+    Hypothesis inj_hashTuple : injective hashTuple.
+    Hypothesis hashTuple_neq_error : forall s, hashTuple s == herror = false.
+    Hypothesis hashTuple_neq_init : forall s, hashTuple s == h0 = false.
 
     Implicit Type trm : term I B L.
 
@@ -68,417 +72,16 @@ Section IsoCan.
     Lemma by_perf_hash trm (o : h) (eqb : hashTerm trm == o) : hashTerm trm = o.
     Proof. apply /eqP. apply eqb. Qed.
 
-    Definition hterm := term I (hash B) L.
-
-    (* should this be a coercion? let's see *)
-    Definition term_of_hterm (ht : hterm) : term I B L :=
-      match ht with
-      |Iri i => Iri i
-      |Bnode hb => Bnode (input hb)
-      |Lit l => Lit l
-      end.
-
-    Definition eqb_trm_hi trm (ht : hterm) : bool := trm == (term_of_hterm ht).
-
-    Definition eqb_b_hterm b (ht : hterm) : bool :=
-      if ht is Bnode hb then b == (input hb) else false.
-
-    Definition htriple := triple I (hash B) L.
-
-    Definition has_term_triple trm (trpl : htriple) : option hterm :=
-      let (s,p,o,_,_) := trpl in
-      if eqb_trm_hi trm s then Some s
-      else if eqb_trm_hi trm p then Some p
-           else if eqb_trm_hi trm o then Some o
-                else None.
-
-    Definition is_some {T : Type} (ot : option T) : bool :=
-      match ot with Some _ => true | None => false end.
-
-    Definition hgraph := rdf_graph I (hash B) L.
-
-    Definition get t (g : hgraph) : option hterm :=
-      let otrs := (map (has_term_triple t) (graph g)) in
-      head None (filter is_some otrs).
-
-    Definition lookup_hash (hb : hterm) : option (hash B) :=
-      if hb is Bnode hin then some hin else None.
-
-    Definition lookup_hash_default (hb : hterm) : h :=
-      if hb is Bnode hin then current_hash hin else herror.
-
-    Section Partition.
-
-      Definition eq_hash (b1 b2 : hterm) : bool :=
-        match (lookup_hash b1), (lookup_hash b2) with
-        | Some hin1, Some hin2 => current_hash hin1 == current_hash hin2
-        | _,_ => false
-        end.
-
-      Lemma eq_hash_refl b : is_bnode b -> eq_hash b b.
-      Proof. rewrite /eq_hash /lookup_hash => isb. case: b isb; rewrite //.
-      Qed.
-
-      (* change for finset *)
-      Fixpoint partitionate (f : hterm -> bool) (s : seq hterm) : seq hterm * seq hterm :=
-        match s with
-        | nil => (nil, nil)
-        | x :: tl => let (g,d) := partitionate f tl in
-                     if f x then (x::g,d) else (g,x::d)
-        end.
-
-      (* should be parameterized by a hgraph
-         part shoud be the finset of (hash B) that shares hash in g *)
-      Definition part := seq (hash B).
-
-      (* the finset of parts in g *)
-      Definition partition := seq part.
-
-      Fixpoint someT_to_T {T : Type} (os : seq (option T)) : seq T :=
-        match os with
-        | nil => nil
-        | Some t :: oss => t :: someT_to_T oss
-        | None :: oss => someT_to_T oss
-        end.
-
-      Definition mkPartition (g : hgraph) : partition :=
-        let bnodes := (bnodes g) in
-        let equiv := (fun b => (fun t=> eq_hash b t)) in
-        (* undup up to permutation *)
-        let P := undup (map (fun b=> (partitionate (equiv b) bnodes).1 ) bnodes) in
-        let ohs := map (fun bs => map lookup_hash bs) P in
-        map someT_to_T ohs.
-
-      Definition is_trivial (p : part) : bool :=
-        size p == 1%N.
-
-      Definition is_non_trivial (p : part) : bool :=
-        ~~ is_trivial p.
-
-      Definition is_fine (P : partition) : bool :=
-        all is_trivial P.
-
-      Definition is_coarse (P : partition) : bool :=
-        size P == 1%N.
-
-      Definition is_intermediate (P : partition) :=
-        ~~ is_fine P && ~~ is_coarse P.
-
-    End Partition.
-
     Definition init_bnode (b : B) : (hash B) :=
       mkHinput b h0.
 
-    (* Algorithm 1, lines 2-8
-       initializes every blank node with a known default name *)
-    Definition init_hash (g : rdf_graph _ _ _) : hgraph :=
-      relabeling init_bnode g.
-
-    Hypothesis to_string : h -> B.
-    Hypothesis inj_to_string : injective to_string.
-
-    Definition label_bnode (hb : (hash B)) : B :=
-      to_string (current_hash hb).
-
-    Definition label_term (htrm : hterm) : term I B L :=
-      relabeling_term label_bnode htrm.
-
-    Definition label_triple ht : triple I B L :=
-      relabeling_triple label_bnode ht.
-
-    Definition label (g : hgraph) : rdf_graph I B L :=
-      relabeling label_bnode g.
-
-    (* assumes order and no dup in parts *)
-    Definition cmp_part (p1 p2 : part) : bool :=
-      all2 (fun b1 b2 => input b1 == input b2) p1 p2.
-
-    (* assumes order and no dup in partition *)
-    (* answers true if every part in the partition of g is equal to the respective part in h *)
-    Definition cmp_partition (g h: hgraph) : bool :=
-      let Pg := mkPartition g in
-      let Ph := mkPartition h in
-      all2 (fun p1 p2 => cmp_part p1 p2) Pg Ph.
-
-
-    Variable hashBag : seq h -> h.
-    Hypothesis hashBag_assoc : forall (l1 l2 l3: seq h),
-        hashBag ([:: hashBag (l1 ++ l2)] ++ l3) = hashBag (l1 ++ [:: hashBag (l2 ++ l3)]).
-    Hypothesis hashBag_comm : forall (l1 l2: seq h),
-        hashBag (l1 ++ l2) = hashBag (l2 ++ l1).
-
-    Variable hashTuple : seq h -> h.
-    Hypothesis hashTuple_neq_init : forall s, hashTuple s == h0 = false.
-    Hypothesis hashTuple_neq_error : forall s, hashTuple s == herror = false.
-    Lemma hasTuple_neq_errorP s: hashTuple s = herror -> False.
-    Proof. by apply /eqP; rewrite /negb hashTuple_neq_error. Qed.
-
-    Hypothesis inj_hashTuple : injective hashTuple.
-
-    Definition term_hash (trm : hterm) : h :=
-      match trm with
-      | Iri x | Lit x => hashTerm (term_of_hterm trm)
-      | Bnode hb => current_hash hb
-      end.
-
-    (* updates the current hash of b by b' in all the ocurrences
-       in g *)
-    Definition replace_bnode (b b': hash B) (g : hgraph) : hgraph :=
-      relabeling (fun a_hash => if a_hash == b then b' else a_hash) g.
-
-    Definition cmp_bnode (b : B) (ht : hterm) : bool :=
-      match ht with
-      | Bnode hin => b == (input hin)
-      | _ => false
-      end.
-
-    Definition lookup_bnode_in_triple (b : B) (t : htriple) : option hterm :=
-      let (s,p,o,_,_) := t in
-      if cmp_bnode b s then Some s
-      else if cmp_bnode b p then Some p
-           else if cmp_bnode b o then Some o else None.
-
-    Definition lookup_bnode_in_graph (g : hgraph) (b : B) : option hterm :=
-      let otrms := map (lookup_bnode_in_triple b) g in
-      head None (filter is_some otrms).
-
-    Definition lookup_bnode_in_graph' (g : hgraph) (b : B) : option hterm :=
-      match (filter (cmp_bnode b) (bnodes g)) with
-      | nil => None
-      | hb :: _ => Some hb
-      end.
-
-    Definition lookup_bnode_in_graph_default (g : hgraph) (b : B) : h :=
-      if lookup_bnode_in_graph g b is Some trm then term_hash trm else herror.
-
-    Definition new_hash (s p o : hterm) gacc hldr : option ((hash B) * (hash B)) :=
-      if s is Bnode hb
-      then
-        let c := hashTuple [:: (term_hash o) ; (term_hash p) ; hldr] in
-        let b_curr := lookup_bnode_in_graph_default gacc (input hb) in
-        Some (hb,(mkHinput (input hb) (hashBag [:: c ; b_curr ])))
-      else None.
-
-    Definition new_hash_fwd (s p o: hterm) gacc : option ((hash B) * (hash B)) :=
-      new_hash s p o gacc hfwd.
-
-    Definition new_hash_bwd (s p o : hterm) gacc : option ((hash B) * (hash B)) :=
-      new_hash o p s gacc hbwd.
-
-    (* Algorithm 1, lines 12-17
-       update the hashes of blank nodes using the neighborhood
-       it hashes differently outgoing edges from incoming ones *)
-    Definition update_bnodes (g : hgraph) : hgraph :=
-      let fix help g gacc hf :=
-        match g with
-        | nil => gacc
-        | cons t ts => let (s,p,o,_,_) := t : htriple in
-                       let newhash := hf s p o gacc in
-                       if newhash is Some (hb,hb')
-                       then let gacc' := replace_bnode hb hb' gacc in
-                            help ts gacc' hf
-                       else help ts gacc hf
-        end in
-      let g_fwd := help g g new_hash_fwd in
-      help g g_fwd new_hash_bwd.
-
-    (* Algorithm 1, lines 9-18
-       the iteration: computes the update of blank nodes until
-           - the partition is fine
-           - the partition did not change with respect to the previous one
-     *)
-    Fixpoint iterate (g : hgraph) (fuel : nat) : hgraph :=
-      match fuel with
-      | O => g
-      | S n' =>
-          let h := update_bnodes g in
-          if cmp_partition g h || is_fine (mkPartition h) then h else
-            iterate h n'
-      end.
-
-
-    Definition hashNodes_initialized (g : hgraph) : hgraph :=
-      iterate g (size (graph g)).
-
-    (* need the lemma stating hashNodes terminates without
-       getting out of fuel *)
-    (* Algorithm 1*)
-    Definition hashNodes (g : rdf_graph _ _ _) : hgraph :=
-      hashNodes_initialized (init_hash g).
-
-    (* Definition 4.6 ≡ ~G *)
-    Definition reachability_rel (g : hgraph) (t1 t2 : htriple) : bool :=
-      let (s1, _, o1, _, _) := t1 in
-      let (s2, _, o2, _, _) := t2 in
-      let s1s2 := (s1 == s2) && is_bnode s1 in
-      let s1o2 := (s1 == o2) && is_bnode s1 in
-      let o1s2 := (o1 == s2) && is_bnode o1 in
-      let o1o2 := (o1 == o2) && is_bnode o1 in
-      s1s2 || s1o2 || o1s2 || o1o2.
-
-    (* Algorithm 2, line 2:
-       computes the connected components based on definition 4.6 (~G)
-     *)
-    Definition blank_node_split (t u v : Type) (g : rdf_graph t u v) : seq (rdf_graph t u v).
-    Proof.
-    (* compute the graph G,
-         where V := g and
-         (t,u) : (triple I B L * triple I B L) \in E iff
-         [:: t ; u] is graph and bnodes(t) ∩ bnodes(u) ≠ ϕ
-
-       Then compute the connected componens using reachability rel*)
-    Admitted.
-
-    (* The graph that contains all (and only the) ground triples of G *)
-    Definition ground_split {t u v : Type} (g : rdf_graph t u v) : rdf_graph t u v :=
-      let groundTriples := filter (fun t => is_ground_triple t) g in
-      mkRdfGraph groundTriples.
-
-    Lemma merge_split {t u v : Type} (g : rdf_graph t u v) :
-      merge_rdf_graph (merge_seq_rdf_graph (blank_node_split g)) (ground_split g) = g.
-    Admitted.
-
-    (* Algorithm 2 *)
-    Definition hashBnodesPerSplit (g : hgraph) : hgraph :=
-      let splitG := blank_node_split g in
-      foldr (@merge_rdf_graph _ _ _) (empty_rdf_graph _ _ _) splitG.
+    Lemma inj_init_bnode : injective init_bnode.
+    Proof. by move=> x y; rewrite /init_bnode=> [[]] ->. Qed.
 
     (* Algorithm 3, line 13
        hashes b incorporating an arbitrary hash hmark *)
     Definition mark_hash (b : hash B) : hash B :=
       mkHinput (input b) (hashTuple [:: (current_hash b) ; hmark]).
-
-    Definition mark_bnode (b : hterm) : hterm :=
-      match b with
-      | Iri i| Lit i => Bnode (mkHinput b0 herror)
-      | Bnode hb=> Bnode (mark_hash hb)
-      end.
-
-    (* algorithm 3, lines 9-10
-       chooses the canonical part which is not fine *)
-    Fixpoint choose_part (P : partition) : part :=
-      match P with
-      | nil => nil (* FIXME: is this the good way to do it? *)
-      | cons p t => if is_trivial p then choose_part t else p
-      end.
-
-    (* Algorithm 3, lines 13-14 when color refine is hashBnodes_initialized.
-       b is_bnode *)
-    Definition distinguishBnode g (color_refine : hgraph -> hgraph ) (b : hash B) : hgraph :=
-      let b' := mark_hash b in
-      let g' := replace_bnode b b' g in
-      color_refine g'.
-
-    (* choose canonical graph from sequence of graphs that have fine partitions *)
-    Definition choose_graph (gs : seq hgraph) : hgraph :=
-      if insub gs : {? x | all (is_fine \o mkPartition) x} is Some _
-      then foldl Order.max (mkRdfGraph [::]) gs
-      else mkRdfGraph [::].
-
-    (* give partition and proof that partition is not fine *)
-    (* or compute it again ... *)
-    (* Algorithm 3, function distinguish, lines 9-20
-       lines 16-18 were moved to a higher level: should consume more space
-       FIXME just call distinguish_ with not fine partitions so
-       is not needed to repeat the question *)
-    Fixpoint distinguish_ g (color : hgraph -> hgraph) (fuel:nat) : hgraph :=
-      match fuel with
-      | O => g
-      | S n' =>
-          let P := mkPartition g in
-          if is_fine P then g
-          else
-            let p := choose_part P in
-            let gs := map (distinguishBnode g color) p in
-            let just_fine := (fun g: hgraph =>
-                                if is_fine (mkPartition g) then g
-                                else distinguish_ g color n') in
-            choose_graph (map just_fine gs)
-      end.
-
-    (* Algorithm 3, function distinguish
-       when color_refine is hashBnodes_initialized *)
-    Definition distinguish g (color_refine : hgraph -> hgraph) : hgraph :=
-      distinguish_ g color_refine (size g).
-
-    (* FIXME replace by padding function
-     if ht in g then lookup in a finfun else
-     just the input of the hterm *)
-    Definition build_mapping_from_graph (g : hgraph) : B -> B :=
-      let f := fun ht mapping =>
-                 (fun b =>
-                    if (input ht) == b
-                    then (to_string (current_hash ht))
-                    else mapping b) in
-      foldr f id (get_b g).
-
-    Definition build_mapping_from_graph' (g : hgraph) : B -> B :=
-      let bns := bnodes g in
-      fun b =>
-        let p := eqb_b_hterm b in
-        let default := (Bnode (mkHinput b herror)) in
-        if has p bns then
-          let the_bnode := nth default bns (find p bns) in
-          to_string (lookup_hash_default the_bnode)
-        else b.
-
-    Definition map_fintype (T U: eqType) (s : seq T) (f : T -> U) (arg : seq_sub s) : seq_sub (map f s).
-    Proof. suffices: f (ssval arg) \in (map f s). by apply SeqSub.
-           by apply (map_f f); apply (ssvalP arg).
-    Qed.
-
-    Definition build_finfun_from_graph (g : hgraph) :
-      (seq_sub (bnodes g)) -> (seq_sub (map label_term (bnodes g))).
-    Proof. apply map_fintype. Qed.
-
-    Definition build_mapping_from_seq (trms : seq hterm) : B -> B :=
-      fun b =>
-        if has (eqb_b_hterm b) trms then
-          let the_bnode := nth (Bnode (mkHinput b herror)) trms (find (eqb_b_hterm b) trms) in
-          to_string (lookup_hash_default the_bnode)
-        else
-          b.
-
-    Fixpoint app_n (T: Type)(f : T -> T) (x : T) (n:nat) :=
-      match n with
-      | O => x
-      | S n' => f (app_n f x n')
-      end.
-
-    Definition k_distinguish bns : seq (term I (hash B) L) :=
-      let fix help bns n :=
-        match bns with
-        | nil => nil
-        | trm :: trms => app_n mark_bnode trm n :: help trms (S n)
-        end in
-      help bns 0.
-
-    Definition mapi {A B : Type} (f : A -> nat ->  B) (s : seq A) : seq B :=
-      map (fun an => (f an.1) an.2) (zip s (iota 0 (size s))).
-
-    Definition ak_mapping (g : rdf_graph I B L) : seq hterm :=
-      let bns := bnodes (init_hash g) in
-      mapi (app_n mark_bnode) bns.
-
-    Definition fun_to_fin (T : eqType) (s : seq T) (f : T -> T) : seq_sub s -> T:=
-      fun s0=> let (ssval,_) := s0 in (f ssval).
-
-    Lemma inj_init_bnode : injective init_bnode.
-    Proof. by move=> x y; rewrite /init_bnode=> [[]] ->. Qed.
-
-    Lemma mark_hash_init b g : Bnode b \in bnodes (init_hash g) -> current_hash b = h0.
-    Proof. rewrite /bnodes/init_hash -filter_undup mem_filter /=.
-           by rewrite undup_terms (terms_relabeled g inj_init_bnode)=> /map_inv[[] // ?]=> [[]] ->.
-    Qed.
-
-    Lemma app_n_mark_bnode g b n:
-      Bnode b \in bnodes (init_hash g) ->
-                  app_n mark_bnode (Bnode b) n =
-                    Bnode (app_n mark_hash (mkHinput (input b) h0) n).
-    Proof. move=> /mark_hash_init b_hash.
-           elim n=> [| n' IHn]; last by rewrite /= IHn.
-           by rewrite /=; f_equal; case: b b_hash=> /= [[]] ? ? /= ->.
-    Qed.
 
     Lemma mark_hash_idem_inj b1 b2:
       mark_hash (mark_hash b1) == mark_hash (mark_hash b2) ->
@@ -495,30 +98,7 @@ Section IsoCan.
            app_n mark_hash (mkHinput (input b2) h0) n).
     Proof. elim: n=> [/=| n' IHn].
            case b1; case b2=> [[a b] [a' b']]; first by rewrite eq_i_ch/==> [/andP [/eqP ->]]; rewrite !eqxx.
-           by move=> /=/mark_hash_idem_inj/IHn => /andP [-> /eqP ->] /=. 
-    Qed.
-
-    Lemma inj_mark_bnode g: {in (bnodes g), injective mark_bnode}.
-    Proof. move=> x in_bns y.
-           case: x in_bns; case y=> x' y'; rewrite ?i_in_bnodes ?l_in_bnodes // => in_bns /=
-               => [[]] i_eq /eqP; rewrite ?hashTuple_neq_error //
-               => /eqP/inj_hashTuple []=> ch_eq.
-           by f_equal; apply /eqP; rewrite eq_i_ch i_eq ch_eq !eqxx.
-    Qed.
-
-    Lemma eq_appn_init_eq_num b1 b2 g (b1in_bns : Bnode b1 \in bnodes (init_hash g))
-      (b2in_bns : Bnode b2 \in bnodes (init_hash g)) n m :
-      (app_n mark_bnode (Bnode b1) n) =
-        (app_n mark_bnode (Bnode b2) m) ->
-      n = m.
-    Proof.
-      have b1_hash:  current_hash b1 = h0. by apply: mark_hash_init b1in_bns.
-      have b2_hash:  current_hash b2 = h0. by apply: mark_hash_init b2in_bns.
-      rewrite (app_n_mark_bnode n b1in_bns) (app_n_mark_bnode m b2in_bns)=> [appn_eq].
-      elim: n m appn_eq=> [// m | n' IHn m]; first by case: m=> [//| m' [_ /eqP]]; rewrite eq_sym hashTuple_neq_init.
-      + case: m IHn=> [//| m'] IHn []; first by move=> _ /eqP /=; rewrite hashTuple_neq_init.
-      - move=> eq_i /inj_hashTuple [] eq_ch.
-        by rewrite (IHn m')=> //; f_equal; apply /eqP; rewrite eq_i_ch eq_i eq_ch !eqxx.
+           by move=> /=/mark_hash_idem_inj/IHn => /andP [-> /eqP ->] /=.
     Qed.
 
     Lemma appn_mark_hash_eq_input (b1 b2: hash B) n:
@@ -530,399 +110,755 @@ Section IsoCan.
       by rewrite eq_i_ch /= eqxx Bool.andb_true_r.
     Qed.
 
-    Lemma app_n_mark_eq_bns (b1 b2: hash B) g (b1in_bns : Bnode b1 \in bnodes (init_hash g))
-      (b2in_bns : Bnode b2 \in bnodes (init_hash g)) n:
-      (app_n mark_bnode (Bnode b1) n) == (app_n mark_bnode (Bnode b2) n) ->
-      (@Bnode I (hash B) L b1) == (Bnode b2).
-    Proof.
-      rewrite (app_n_mark_bnode n b1in_bns) (app_n_mark_bnode n b2in_bns)
-              => /eqP [] /eqP /appn_mark_hash_eq_input eq_i.
-      suffices eqbn: b1 = b2. by rewrite eqbn.
-      by apply /eqP; rewrite eq_i_ch eq_i (mark_hash_init b1in_bns) (mark_hash_init b2in_bns) eqxx.
-    Qed.
-
-    Lemma can_app_n_mb_init g b1 b2 (b1_bns : Bnode b1 \in bnodes (init_hash g))
-      (b2_bns : Bnode b2 \in bnodes (init_hash g))
-      n m :
-      app_n mark_bnode (Bnode b1) n = app_n mark_bnode (Bnode b2) m ->
-      (@Bnode I (hash B) L b1 == Bnode b2) && (n == m).
-      move=> /eqP injH.
-      suffices eqnm: n = m.
-      rewrite eqnm in injH *; f_equal; rewrite eqxx Bool.andb_true_r; apply: (app_n_mark_eq_bns b1_bns b2_bns injH).
-      by move/eqP: injH; apply (eq_appn_init_eq_num b1_bns b2_bns).
-    Qed.
-
-
-    Lemma k_mapping_seq_uniq_graph g: uniq (mapi (app_n mark_bnode) (bnodes (init_hash g))).
-    Proof.
-      rewrite /mapi; pose g' := init_hash g.
-      rewrite map_inj_in_uniq; first by apply (zip_uniq_l _ (uniq_bnodes g')).
-      move=> [t n] [u m] /in_zip/andP [tin_bns n_iota] /in_zip/andP [uin_bns m_iota] /= eq_app_n.
-      case: t tin_bns uin_bns eq_app_n; case: u
-          => nt nu; rewrite ?i_in_bnodes ?l_in_bnodes // => nu_bns nt_bns injH.
-      by apply /eqP; rewrite xpair_eqE; apply (can_app_n_mb_init nu_bns nt_bns injH).
-    Qed.
-
-    Lemma k_mapping_seq_uniq_perm_eq g s: perm_eq s (bnodes (init_hash g)) -> uniq (mapi (app_n mark_bnode) s).
-    Proof. rewrite /mapi perm_sym=> perm_eq. rewrite map_inj_in_uniq. apply uniq_zip_iota.
-           move=> [x1 n] [y1 m] /in_zip/andP [x1_ins n_iniota] /in_zip/andP [y1_ins m_iniota] /=.
-           have : is_bnode x1. apply (in_all x1_ins); rewrite -(perm_all _ perm_eq); apply all_bnodes.
-           have : is_bnode y1. apply (in_all y1_ins); rewrite -(perm_all _ perm_eq); apply all_bnodes.
-           case :y1 x1_ins y1_ins; case x1=> // namey namex y_ins x_ins _ _.
-           have y1_init: Bnode namey \in (bnodes (init_hash g)). rewrite (perm_mem perm_eq). apply y_ins.
-           have x1_init: Bnode namex \in (bnodes (init_hash g)). rewrite (perm_mem perm_eq). apply x_ins.
-           by move=> ?; apply /eqP; rewrite xpair_eqE; apply (can_app_n_mb_init y1_init).
-    Qed.
-
-    Definition k_mapping (g : rdf_graph I B L) : rdf_graph I B L :=
-      let all_maps :=
-        map (mapi (app_n mark_bnode)) (permutations (bnodes (init_hash g))) in
-      let mus := map build_mapping_from_seq all_maps in
-      let isocans := map (fun mu => relabeling mu g) mus in
-      foldl Order.max (mkRdfGraph [::]) isocans.
-
-    Definition isoCanonicalTemplate g (color color_refine: hgraph -> hgraph)
-      p_refining : rdf_graph I B L:=
-      let g' := color (init_hash g) in
-      let P := mkPartition g' in
-      let g_iso := if is_fine P then g' else p_refining g' color_refine in
-      label g_iso.
-
-    (* first approach *)
-    Definition justDistinguish g :=
-      isoCanonicalTemplate g id id distinguish.
-
-    Definition isoCanonicalNoIter g :=
-      isoCanonicalTemplate g update_bnodes update_bnodes distinguish.
-
-    Definition isoCanonicalIter g :=
-      isoCanonicalTemplate g hashNodes_initialized hashNodes_initialized distinguish.
-
-    Definition isoCanonicalise g :=
-      isoCanonicalTemplate g hashBnodesPerSplit hashNodes_initialized distinguish.
-
-    Lemma no_bnodes_same_partition t ts :
-      bnodes_triple t = [::] ->
-      is_fine (mkPartition {| graph := ts |}) ->
-      is_fine (mkPartition {| graph := t :: ts |}).
-    Proof. by rewrite /mkPartition bnodes_cons /bnodes => -> /=; rewrite undup_idem. Qed.
-
-    Lemma eq_hash_refl_singl b g :
-      bnodes g = [:: b] ->
-      (if eq_hash b b then ([:: b], [::]) else ([::], [:: b])).1 = [:: b].
-    Proof. by move=> H; apply b_in_bnode_is_bnode in H; rewrite (eq_hash_refl H). Qed.
-
-    Lemma sing_fine (g : hgraph) (b : hterm): bnodes g = [:: b] -> is_fine (mkPartition g).
-    Proof.
-      case: g b=> g'; elim: g'=> [//| t ts IHts].
-      rewrite bnodes_cons.
-      case t=> s p o; case s; case p; case o=>
-             //; rewrite /bnodes_triple/terms_triple
-             => id id0 id1 sib pii b; rewrite filter_undup ?undup_idem /mkPartition
-             => /= singl; try (move: singl; rewrite /undup_idem bnodes_cons /bnodes_triple /terms_triple filter_undup /= undup_bnodes).
-      (* room for improvement *)
-      + apply no_bnodes_same_partition. by rewrite /bnodes_triple filter_undup. apply (IHts b singl).
-      + apply no_bnodes_same_partition. by rewrite /bnodes_triple filter_undup. apply (IHts b singl).
-      (* =============== *)
-      + case e: (Bnode id \in bnodes {| graph := ts |})=> singl.
-      - by apply (IHts b singl).
-      - by case: singl=> _ -> /=; rewrite eq_hash_refl.
-        (* =============== *)
-        + case: (Bnode id1 \in bnodes {| graph := ts |})=> singl.
-      - by apply (IHts b singl).
-      - by case: singl=> _ -> /=; rewrite eq_hash_refl.
-        (* =============== *)
-        + case: (Bnode id1 \in bnodes {| graph := ts |})=> singl.
-      - by apply (IHts b singl).
-      - by case: singl=> _ -> /=; rewrite eq_hash_refl.
-        (* =============== *)
-        + move: singl.
-          have b_def : (bnodes_triple
-                          {|
-                            subject := Bnode id1;
-                            predicate := Iri id0;
-                            object := Bnode id;
-                            subject_in_IB := sib ;
-                            predicate_in_I := pii
-                          |}) =
-                         (if Bnode id1 \in [:: Bnode id] then [:: Bnode id] else [:: Bnode id1; Bnode id]).
-          move=> ? ?. by rewrite /bnodes_triple /terms_triple filter_undup /=.
-          rewrite bnodes_cons /bnodes_triple filter_undup -b_def -bnodes_cons => singl.
-          rewrite /= -b_def -bnodes_cons singl.
-          have isbb: is_bnode b. by apply (b_in_bnode_is_bnode singl).
-          by rewrite /= (eq_hash_refl isbb); case: b isbb singl.
-    Qed.
-
-    Lemma distinguish_preserves_isomorphism g : iso (justDistinguish g) g.
-    Proof.
-      rewrite /iso/justDistinguish/isoCanonicalTemplate/is_iso.
-      case (is_fine (mkPartition (init_hash g))).
-      case g=> g'. elim g'=> [|t ts ihts].
-      - exists id. split.
-        + by exists id.
-                    + by rewrite relabeling_id.
-                    -
-                      (* need to build μ. and μ bij. *)
-    Admitted.
-
-    Lemma empty_ak_mapping : ak_mapping (mkRdfGraph [::]) = [::]. Proof. by []. Qed.
-
-    Lemma inv_of_ak_mapping g : exists mu,
-        (relabeling mu g) == (relabeling (build_mapping_from_seq (ak_mapping g)) g).
-    Proof. by exists (build_mapping_from_seq (ak_mapping g)). Qed.
-
-
-    Lemma inv_of_perm_ak_mapping g (p : seq hterm) :
-      p \in (permutations (ak_mapping g)) -> (*no need for this*)
-            exists mu, (relabeling mu g) == (relabeling (build_mapping_from_seq p) g).
-    Proof.
-      by exists (build_mapping_from_seq p).
-    Qed.
-
-    Lemma the_μ g :
-      exists f,
-        [seq relabeling mu0 g
-        | mu0 <- [seq build_mapping_from_seq i
-                 | i <- permutations (ak_mapping g)]] =
-
-          map f [seq build_mapping_from_seq i
-                | i <- permutations (ak_mapping g)].
-    Proof. rewrite /= /ak_mapping. elim g=> gs; elim: gs=> [| a t IHts].
-           - by exists (fun g=> relabeling g (mkRdfGraph [::])).
-                       - admit.
-    Admitted.
-
-    Lemma init_hash_nil : init_hash {| graph := [::] |} = {| graph := [::] |}. by []. Qed.
-
-    Lemma relabeling_mu_inv (g : rdf_graph I B L) (fs : seq (B -> B)) mapping :
-      (mapping g) \in (map (fun mu => relabeling mu g) fs) ->
-                      exists (mu : B -> B), relabeling mu g == mapping g.
-    Proof.
-      elim : fs => [| f fs' IHfs]; first by rewrite in_nil.
-      rewrite in_cons; case/orP.
-      + by rewrite eq_sym; exists f.
-      + by move=> /IHfs //.
-    Qed.
-
-    Lemma injection_hterm b (ht : hterm) : eqb_b_hterm b ht -> is_bnode ht.
-    Proof. by case ht. Qed.
-
-    Lemma eqb_b_hterm_trans b b' ht : eqb_b_hterm b ht -> eqb_b_hterm b' ht -> b = b'.
-    Proof. by case: ht=> // name; move=> /eqP -> /eqP ->. Qed.
-
-    Lemma injection_kmap b b' ht s (eb: eqb_b_hterm b ht) (eb': eqb_b_hterm b' ht):
-      (build_mapping_from_seq (mapi (app_n mark_bnode) s) b) =
-        (build_mapping_from_seq (mapi (app_n mark_bnode) s) b').
-    Proof. suffices : b = b'. by move=> ->.
-           by apply (eqb_b_hterm_trans eb eb'). Qed.
-
     Definition mu_extension (mu : B -> B) : (hash B) -> (hash B):=
       fun b => (mkHinput (mu (input b)) (current_hash b)).
 
-    Definition relabeling_hterm (mu : B -> B) ht : hterm :=
-      relabeling_term (mu_extension mu) ht.
-
-    Lemma eqb_b_hterm_relabel f b ht (injF: injective f): (eqb_b_hterm b ht) = (eqb_b_hterm (f b) (relabeling_hterm f ht)).
-    Proof. by case ht=> // name /=; rewrite inj_eq. Qed.
-
-    Lemma has_map s f b (injF: injective f): has (eqb_b_hterm b) s = has (eqb_b_hterm (f b)) (map (relabeling_hterm f) s).
-    Proof. elim: s=> [//|hd tl IHtl] /=.
-           + f_equal; last by rewrite IHtl.
-             by apply eqb_b_hterm_relabel.
-    Qed.
-
-    Lemma lookup_hash_relabeling ht mu: (lookup_hash_default ht) = (lookup_hash_default (relabeling_hterm mu ht)).
-    Proof. by case ht. Qed.
-
-    Lemma map_kmap b n s :
-      (build_mapping_from_seq s b) = n ->
-      (has (eqb_b_hterm b) s) ->
-      forall s' (f : B -> B), injective f -> s' = map (relabeling_hterm f) s ->
-                              (build_mapping_from_seq s' (f b)) = n.
-    Proof.
-      elim: s=> [| hd tl IHtl]; first by rewrite has_nil.
-      move=> beq has_b s'; case: s'=> [//| hd' tl'] f injF [eqhd eqtl].
-      move: IHtl; rewrite /build_mapping_from_seq eqhd eqtl -map_cons -has_map; last by apply injF.
-      rewrite has_b /= -eqb_b_hterm_relabel; last by apply injF. rewrite /= in has_b.
-      case/orP: has_b beq; first by rewrite /build_mapping_from_seq=> H /=; rewrite H; case hd=> // name /=.
-      + rewrite /build_mapping_from_seq /= ; case e: (eqb_b_hterm b hd)
-                => /=; first by move=> _; rewrite -lookup_hash_relabeling.
-        move=> /= has_tl /=; rewrite has_tl=> eq IHtl.
-        have IHtl' := IHtl eq isT tl' f injF eqtl.
-        by rewrite eqtl -has_map ?has_tl in IHtl'; last by apply injF.
-    Qed.
-
-    Lemma has_not_default T (s : seq T) p :
-      has p s -> forall x0 x1,  nth x0 s (find p s) = nth x1 s (find p s).
-    Proof. elim: s=> [//| hd tl IHtl] /= hps x1.
-           by case/orP: hps=> [-> //| /IHtl hptl]; case: (p hd)=> //; apply hptl.
-    Qed.
-
-    Lemma eq_to_fin (T: eqType) (ft ft' : finType)
-      (f : T -> T) (injF: injective f)
-      (funt : ft -> T) (injFt: injective funt)
-      (funt' : T -> ft') (injFt' : injective funt')
-      : exists (f'' : ft -> ft'), injective f''.
-    Proof. exists (fun argT => (funt' (f (funt argT)))).
-           by apply: (inj_comp injFt') (inj_comp injF injFt).
-    Qed.
-
-    Lemma all_kmaps_bijective g : List.Forall (fun mu => bijective mu) [seq build_mapping_from_seq i
-                                                                       | i <- [seq mapi (app_n mark_bnode) i
-                                                                              | i <- permutations (bnodes (init_hash g))]].
-    Proof.
-      have map2Listmap U V (f : U -> V) (s : seq U) : map f s = List.map f s. admit.
-      have nth2Listnth U (d : U) (s : seq U) n : nth d s n = List.nth n s d. admit.
-      have size2Listlength U (s : seq U) : List.length s = size s. admit.
-      rewrite !map2Listmap !List.Forall_map.
-      suffices step s : perm_eq s (bnodes (init_hash g)) -> bijective (build_mapping_from_seq (mapi (app_n mark_bnode) s)).
-      apply/List.Forall_nth=> i d lti. apply: step. rewrite -mem_permutations -nth2Listnth. apply: mem_nth.
-      by rewrite -size2Listlength; apply/ltP.
-      (* by using k_mapping_seq_uniq_perm_eq *)
-      admit.
-    Admitted.
-
-    (* TODO *)
-    (* only way of k_mapping g = [::] -> g = [::]*)
-    Lemma inv_of_k_mapping g : exists mu, (relabeling mu g) == (k_mapping g) /\ bijective mu.
-    Proof.
-      (* FIX ME*)
-      (* have step1 : k_mapping g = mkRdfGraph [::] \/ *)
-      (*                (k_mapping g) \in [seq relabeling mu0 g *)
-      (*                                  | mu0 <- [seq build_mapping_from_seq i *)
-      (*                                           | i <- [seq mapi (app_n mark_bnode) i *)
-      (*                                                  | i <- permutations *)
-      (*                                                           (bnodes (init_hash g))]]]. *)
-      (* rewrite /=. /k_mapping relabeling_id; apply: foldl_op. *)
-      (* case: step1=> [ -> | in_tail ]. *)
-      (* + exists id; split. *)
-      (* - by rewrite relabeling_id. *)
-      (* - exact: id_bij.  *)
-      (*   + have [mu eq_mu_map] : exists mu : B -> B, relabeling mu g == k_mapping g. *)
-      (*     exact: relabeling_mu_inv in_tail. *)
-      (*     exists mu. split; first exact eq_mu_map. *)
-      (*     (* needs mu to have eqType, could be a finfun *) *)
-      (*     have fin_mu : (seq_sub (bnodes g)) -> B. *)
-      (*     Fail move: (finfun (fun b => b)). *)
-      (*     admit. *)
-      (* Fail fin_mu \in in_tail. *)
-    Admitted.
-
-    (* TODO *)
-    (* USES inv_of_k_mapping *)
-    Lemma k_mapping_iso_output : mapping_is_iso k_mapping.
-    Proof. move=> g; case (inv_of_k_mapping g)=> μ [rel_eq_kmap bijmu].
-           exists μ. split. exact: bijmu. by rewrite eq_sym.
-    Qed.
-
-    Lemma max_sym disp (T: porderType disp) : symmetric Order.max.
-    Proof. by move=> x y; rewrite Order.POrderTheory.maxEle Order.POrderTheory.maxElt Order.TotalTheory.leNgt; case: (y < x).
-    Qed.
-
-    Lemma min_sym : symmetric Order.min.
-    Proof. by move=> x y; rewrite Order.POrderTheory.minEle Order.POrderTheory.minElt Order.TotalTheory.leNgt; case: (y < x).
-    Qed.
-
-    Lemma max_distr_foldl disp (T: porderType disp) (l : seq T) (x y : T) :
-      foldl Order.max (Order.max x y) l = Order.max y (foldl Order.max x l).
-    Proof. elim: l=> [//| hd t IHt] /=.
-           (*  Error: The LHS of Order.TotalTheory.leNgt *)
-           (* (_ <= _) *)
-           (* does not match any subterm of the goal *)
-           (* rewrite Order.POrderTheory.maxEle Order.POrderTheory.maxElt Order.TotalTheory.leNgt; case: (y < x). *)
-           (* Error: The LHS of max_sym *)
-           (*     (Order.max _ _) *)
-           (* does not match any subterm of the goal *)
-           (* rewrite max_sym. *)
-    Admitted.
-
-    Lemma foldl_foldl_max disp (T: orderType disp) (l : seq T) (x0 : T) :
-      foldl Order.max x0 l == foldr Order.max x0 l.
-    Proof. elim: l x0=> [//| hd t IHt] x0 /=.
-           have <- :  ((foldl Order.max x0 t) = (foldr Order.max x0 t)). by apply /eqP; apply IHt.
-           by rewrite max_distr_foldl.
-    Qed.
-
-    (* Lemma bnodes_init_hash g : bnodes (init_hash g) = (map (relabeling_term init_bnode) (bnodes g)). *)
-    (* Proof. Admitted. *)
-
-    (* Lemma bnodes_init_hash_relabel g (mu: B -> B): bnodes (init_hash (relabeling mu g)) = (map (relabeling_term init_bnode) (bnodes (relabeling mu g))). *)
-    (* Proof. Admitted. *)
-
-    (* Lemma bnodes_relabel (g: rdf_graph I B L) (mu: B -> B): bnodes (relabeling mu g) = (map (relabeling_term mu) (bnodes g)). *)
-    (* Proof. Admitted. *)
-
-    (* Lemma perm_map (T U: eqType) (s: seq T) (f: T -> U): permutations (map f s) = map (map f) (permutations s). *)
-    (* Proof. Admitted. *)
-
-    Definition relabeling_hgraph (mu : B -> B) (g: hgraph) : hgraph :=
-      relabeling (fun b => (mkHinput (mu (input b)) (current_hash b))) g.
-
-    (* Lemma relabeling_swap_init_bnode g (mu : B -> B) : *)
-    (*   (map (relabeling_term init_bnode) (bnodes (relabeling mu g))) = *)
-    (*     map (relabeling_term (mu_extension mu)) (map (relabeling_term init_bnode) (@bnodes I B L g)). *)
-    (* Admitted. *)
-
-    Lemma eqb_b_hterm_relabeling b ht (mu : B -> B) :
-      eqb_b_hterm b ht ->
-      eqb_b_hterm (mu b) (relabeling_hterm mu ht).
-    Proof. by rewrite /eqb_b_hterm; case: ht=> // ? /eqP -> /=; rewrite eqxx. Qed.
+    Hypothesis to_string : h -> B.
+    Hypothesis inj_to_string : injective to_string.
+    Definition label_bnode (hb : (hash B)) : B :=
+      to_string (current_hash hb).
 
 
-    Lemma k_mapping_dont_manipulate_names : (dt_names k_mapping).
-    Proof.
-      rewrite /dt_names=> g μ bijmu.
-      case g=> g'; rewrite /k_mapping.
-      suffices ->:
-        [seq relabeling mu {| graph := g' |}
-        | mu <- [seq build_mapping_from_seq i
+    Section Hterms.
+
+      Definition hterm := term I (hash B) L.
+
+      (* should this be a coercion? let's see *)
+      Definition term_of_hterm (ht : hterm) : term I B L :=
+        match ht with
+        | Iri i => Iri i
+        | Bnode hb => Bnode (input hb)
+        | Lit l => Lit l
+        end.
+
+      Definition eqb_trm_hi trm (ht : hterm) : bool := trm == (term_of_hterm ht).
+
+      Definition eqb_b_hterm b (ht : hterm) : bool :=
+        if ht is Bnode hb then b == (input hb) else false.
+
+      Lemma eqb_b_hterm_is_bnode b (ht : hterm) : eqb_b_hterm b ht -> is_bnode ht.
+      Proof. by case ht. Qed.
+
+      Lemma eqb_b_hterm_trans b b' ht : eqb_b_hterm b ht -> eqb_b_hterm b' ht -> b = b'.
+      Proof. by case: ht=> // name; move=> /eqP -> /eqP ->. Qed.
+
+      Definition lookup_hash (hb : hterm) : option (hash B) :=
+        if hb is Bnode hin then some hin else None.
+
+      Definition lookup_hash_default (hb : hterm) : h :=
+        if hb is Bnode hin then current_hash hin else herror.
+
+      Definition eq_hash (b1 b2 : hterm) : bool :=
+        match (lookup_hash b1), (lookup_hash b2) with
+        | Some hin1, Some hin2 => current_hash hin1 == current_hash hin2
+        | _,_ => false
+        end.
+
+      Lemma eq_hash_refl b : is_bnode b -> eq_hash b b.
+      Proof. by rewrite /eq_hash /lookup_hash ; case: b. Qed.
+
+      Lemma eq_hash_refl_singl b g :
+        bnodes g = [:: b] ->
+        (if eq_hash b b then ([:: b], [::]) else ([::], [:: b])).1 = [:: b].
+      Proof. by move=> H; apply b_in_bnode_is_bnode in H; rewrite (eq_hash_refl H). Qed.
+
+      Definition label_term (htrm : hterm) : term I B L :=
+        relabeling_term label_bnode htrm.
+
+      Definition term_hash (trm : hterm) : h :=
+        match trm with
+        | Iri x | Lit x => hashTerm (term_of_hterm trm)
+        | Bnode hb => current_hash hb
+        end.
+
+      Definition cmp_bnode (b : B) (ht : hterm) : bool :=
+        match ht with
+        | Bnode hin => b == (input hin)
+        | _ => false
+        end.
+
+      Definition mark_bnode (b : hterm) : hterm :=
+        match b with
+        | Iri i| Lit i => Bnode (mkHinput b0 herror)
+        | Bnode hb=> Bnode (mark_hash hb)
+        end.
+
+      Lemma inj_mark_bnode g: {in (bnodes g), injective mark_bnode}.
+      Proof. move=> x in_bns y.
+             (* with just x in bnodes? and not y? *)
+             case: x in_bns; case y=> x' y'; rewrite ?i_in_bnodes ?l_in_bnodes // => in_bns /=
+                 => [[]] i_eq /eqP; rewrite ?hashTuple_neq_error //
+                 => /eqP/inj_hashTuple []=> ch_eq.
+             by f_equal; apply /eqP; rewrite eq_i_ch i_eq ch_eq !eqxx.
+      Qed.
+
+      Definition relabeling_hterm (mu : B -> B) ht : hterm :=
+        relabeling_term (mu_extension mu) ht.
+
+      Lemma lookup_hash_relabeling ht mu: (lookup_hash_default ht) = (lookup_hash_default (relabeling_hterm mu ht)).
+      Proof. by case ht. Qed.
+
+      Lemma eqb_b_hterm_relabel f b ht (injF: injective f): (eqb_b_hterm b ht) = (eqb_b_hterm (f b) (relabeling_hterm f ht)).
+      Proof. by case ht=> // name /=; rewrite inj_eq. Qed.
+
+      Lemma has_map s f b (injF: injective f): has (eqb_b_hterm b) s = has (eqb_b_hterm (f b)) (map (relabeling_hterm f) s).
+      Proof. elim: s=> [//|hd tl IHtl] /=.
+             + f_equal; last by rewrite IHtl.
+               by apply eqb_b_hterm_relabel.
+      Qed.
+
+
+    End Hterms.
+
+    Section Htriple.
+
+      Definition htriple := triple I (hash B) L.
+
+      Definition has_term_triple trm (trpl : htriple) : option hterm :=
+        match (filter (eqb_trm_hi trm) (terms_triple trpl)) with
+        | nil => None
+        | t :: ts => Some t
+        end.
+
+      Definition label_triple ht : triple I B L :=
+        relabeling_triple label_bnode ht.
+
+      Definition lookup_bnode_in_triple (b : B) (t : htriple) : option hterm :=
+        match (filter (cmp_bnode b) (terms_triple t)) with
+        | nil => None
+        | t :: ts => Some t
+        end.
+
+
+    End Htriple.
+
+    Section Hgraph.
+
+      Definition hgraph := rdf_graph I (hash B) L.
+
+      Definition get t (g : hgraph) : option hterm :=
+        let otrs := (map (has_term_triple t) (graph g)) in
+        head None (filter is_some otrs).
+
+      (* Algorithm 1, lines 2-8
+       initializes every blank node with a known default name *)
+      Definition init_hash (g : rdf_graph _ _ _) : hgraph :=
+        relabeling init_bnode g.
+
+      Lemma init_hash_nil : init_hash {| graph := [::] |} = {| graph := [::] |}. by []. Qed.
+
+      Lemma init_hash_h0 b g : Bnode b \in bnodes (init_hash g) -> current_hash b = h0.
+      Proof. rewrite /bnodes/init_hash -filter_undup mem_filter /=.
+             by rewrite undup_terms (terms_relabeled g inj_init_bnode)=> /map_inv[[] // ?]=> [[]] ->.
+      Qed.
+
+      (* todo *)
+      (* Lemma bnodes_init_hash g : bnodes (init_hash g) = (map (relabeling_term init_bnode) (bnodes g)). *)
+      (* Proof. elim g=> g'; elim: g'=> [//| [s p o sib pii] ts IHts]. *)
+      (*        rewrite !bnodes_cons. *)
+      (*        rewrite !undup_cat. *)
+      (*        rewrite map_cat. *)
+      (*        f_equal. admit. *)
+      (*        by rewrite !undup_bnodes IHts. *)
+      (* Admitted. *)
+
+      (* Lemma bnodes_init_hash_relabel g (mu: B -> B): bnodes (init_hash (relabeling mu g)) = (map (relabeling_term init_bnode) (bnodes (relabeling mu g))). *)
+      (* Proof. Admitted. *)
+
+      Lemma mark_bnode_init_hash_mark_hash g b n:
+        Bnode b \in bnodes (init_hash g) ->
+                    app_n mark_bnode (Bnode b) n =
+                      Bnode (app_n mark_hash (mkHinput (input b) h0) n).
+      Proof. move=> /init_hash_h0 b_hash.
+             elim n=> [| n' IHn]; last by rewrite /= IHn.
+             by rewrite /=; f_equal; case: b b_hash=> /= [[]] ? ? /= ->.
+      Qed.
+
+      Lemma eq_appn_init_eq_num b1 b2 g (b1in_bns : Bnode b1 \in bnodes (init_hash g))
+        (b2in_bns : Bnode b2 \in bnodes (init_hash g)) n m :
+        (app_n mark_bnode (Bnode b1) n) =
+          (app_n mark_bnode (Bnode b2) m) ->
+        n = m.
+      Proof.
+        have b1_hash:  current_hash b1 = h0. by apply: init_hash_h0 b1in_bns.
+        have b2_hash:  current_hash b2 = h0. by apply: init_hash_h0 b2in_bns.
+        rewrite (mark_bnode_init_hash_mark_hash n b1in_bns) (mark_bnode_init_hash_mark_hash m b2in_bns)=> [appn_eq].
+        elim: n m appn_eq=> [// m | n' IHn m]; first by case: m=> [//| m' [_ /eqP]]; rewrite eq_sym hashTuple_neq_init.
+        + case: m IHn=> [//| m'] IHn []; first by move=> _ /eqP /=; rewrite hashTuple_neq_init.
+        - move=> eq_i /inj_hashTuple [] eq_ch.
+          by rewrite (IHn m')=> //; f_equal; apply /eqP; rewrite eq_i_ch eq_i eq_ch !eqxx.
+      Qed.
+
+      Lemma app_n_mark_eq_bns (b1 b2: hash B) g (b1in_bns : Bnode b1 \in bnodes (init_hash g))
+        (b2in_bns : Bnode b2 \in bnodes (init_hash g)) n:
+        (app_n mark_bnode (Bnode b1) n) == (app_n mark_bnode (Bnode b2) n) ->
+        (@Bnode I (hash B) L b1) == (Bnode b2).
+      Proof.
+        rewrite (mark_bnode_init_hash_mark_hash n b1in_bns) (mark_bnode_init_hash_mark_hash n b2in_bns)
+                => /eqP [] /eqP /appn_mark_hash_eq_input eq_i.
+        suffices eqbn: b1 = b2. by rewrite eqbn.
+        by apply /eqP; rewrite eq_i_ch eq_i (init_hash_h0 b1in_bns) (init_hash_h0 b2in_bns) eqxx.
+      Qed.
+
+      Lemma can_app_n_mb_init g b1 b2 (b1_bns : Bnode b1 \in bnodes (init_hash g))
+        (b2_bns : Bnode b2 \in bnodes (init_hash g))
+        n m :
+        app_n mark_bnode (Bnode b1) n = app_n mark_bnode (Bnode b2) m ->
+        (@Bnode I (hash B) L b1 == Bnode b2) && (n == m).
+        move=> /eqP injH.
+        suffices eqnm: n = m.
+        rewrite eqnm in injH *; f_equal; rewrite eqxx Bool.andb_true_r; apply: (app_n_mark_eq_bns b1_bns b2_bns injH).
+        by move/eqP: injH; apply (eq_appn_init_eq_num b1_bns b2_bns).
+      Qed.
+
+      Definition label (g : hgraph) : rdf_graph I B L :=
+        relabeling label_bnode g.
+
+      (* updates the current hash of b by b' in all the ocurrences
+       in g *)
+      Definition replace_bnode (b b': hash B) (g : hgraph) : hgraph :=
+        relabeling (fun a_hash => if a_hash == b then b' else a_hash) g.
+
+      Definition lookup_bnode_in_graph (g : hgraph) (b : B) : option hterm :=
+        let otrms := map (lookup_bnode_in_triple b) g in
+        head None (filter is_some otrms).
+
+      Definition lookup_bnode_in_graph' (g : hgraph) (b : B) : option hterm :=
+        match (filter (cmp_bnode b) (bnodes g)) with
+        | nil => None
+        | hb :: _ => Some hb
+        end.
+
+      Definition lookup_bnode_in_graph_default (g : hgraph) (b : B) : h :=
+        if lookup_bnode_in_graph g b is Some trm then term_hash trm else herror.
+
+      (* FIXME replace by padding function
+     if ht in g then lookup in a finfun else
+     just the input of the hterm *)
+      Definition build_mapping_from_graph (g : hgraph) : B -> B :=
+        let f := fun ht mapping =>
+                   (fun b =>
+                      if (input ht) == b
+                      then (to_string (current_hash ht))
+                      else mapping b) in
+        foldr f id (get_b g).
+
+      Definition build_mapping_from_graph' (g : hgraph) : B -> B :=
+        let bns := bnodes g in
+        fun b =>
+          let p := eqb_b_hterm b in
+          let default := (Bnode (mkHinput b herror)) in
+          if has p bns then
+            let the_bnode := nth default bns (find p bns) in
+            to_string (lookup_hash_default the_bnode)
+          else b.
+
+      Definition build_finfun_from_graph (g : hgraph) :
+        (seq_sub (bnodes g)) -> (seq_sub (map label_term (bnodes g))).
+      Proof. apply map_fintype. Qed.
+
+      Definition relabeling_hgraph (mu : B -> B) (g: hgraph) : hgraph :=
+        relabeling (fun b => (mkHinput (mu (input b)) (current_hash b))) g.
+
+      Lemma eqb_b_hterm_relabeling b ht (mu : B -> B) :
+        eqb_b_hterm b ht ->
+        eqb_b_hterm (mu b) (relabeling_hterm mu ht).
+      Proof. by rewrite /eqb_b_hterm; case: ht=> // ? /eqP -> /=; rewrite eqxx. Qed.
+
+
+    End Hgraph.
+
+    Section Partition.
+
+      (* change for finset *)
+      Fixpoint partitionate (f : hterm -> bool) (s : seq hterm) : seq hterm * seq hterm :=
+        match s with
+        | nil => (nil, nil)
+        | x :: tl => let (g,d) := partitionate f tl in
+                     if f x then (x::g,d) else (g,x::d)
+        end.
+
+      (* should be parameterized by a hgraph
+         part shoud be the finset of (hash B) that shares hash in g *)
+      Definition part := seq (hash B).
+
+      (* the finset of parts in g *)
+      Definition partition := seq part.
+
+      Definition mkPartition (g : hgraph) : partition :=
+        let bnodes := (bnodes g) in
+        let equiv := (fun b => (fun t=> eq_hash b t)) in
+        (* undup up to permutation *)
+        let P := undup (map (fun b=> (partitionate (equiv b) bnodes).1 ) bnodes) in
+        let ohs := map (fun bs => map lookup_hash bs) P in
+        map someT_to_T ohs.
+
+      Definition is_trivial (p : part) : bool :=
+        size p == 1%N.
+
+      Definition is_non_trivial (p : part) : bool :=
+        ~~ is_trivial p.
+
+      (* assumes order and no dup in parts *)
+      Definition cmp_part (p1 p2 : part) : bool :=
+        all2 (fun b1 b2 => input b1 == input b2) p1 p2.
+
+      Definition is_fine (P : partition) : bool :=
+        all is_trivial P.
+
+      Definition is_coarse (P : partition) : bool :=
+        size P == 1%N.
+
+      Definition is_intermediate (P : partition) :=
+        ~~ is_fine P && ~~ is_coarse P.
+
+      (* assumes order and no dup in partition *)
+      (* answers true if every part in the partition of g is equal to the respective part in h *)
+      Definition cmp_partition (g h: hgraph) : bool :=
+        let Pg := mkPartition g in
+        let Ph := mkPartition h in
+        all2 (fun p1 p2 => cmp_part p1 p2) Pg Ph.
+
+      (* algorithm 3, lines 9-10
+       chooses the canonical part which is not trivial *)
+      Fixpoint choose_part (P : partition) : part :=
+        match P with
+        | nil => nil (* FIXME: is this the good way to do it? *)
+        | cons p t => if is_trivial p then choose_part t else p
+        end.
+
+      (* choose canonical graph from sequence of graphs that have fine partitions *)
+      Definition choose_graph (gs : seq hgraph) : hgraph :=
+        if insub gs : {? x | all (is_fine \o mkPartition) x} is Some _
+        then foldl Order.max (mkRdfGraph [::]) gs
+        else mkRdfGraph [::].
+
+      Lemma no_bnodes_same_partition t ts :
+        bnodes_triple t = [::] ->
+        is_fine (mkPartition {| graph := ts |}) ->
+        is_fine (mkPartition {| graph := t :: ts |}).
+      Proof. by rewrite /mkPartition bnodes_cons /bnodes => -> /=; rewrite undup_idem. Qed.
+
+      Lemma sing_fine (g : hgraph) (b : hterm): bnodes g = [:: b] -> is_fine (mkPartition g).
+      Proof.
+        case: g b=> g'; elim: g'=> [//| t ts IHts].
+        rewrite bnodes_cons.
+        case t=> s p o; case s; case p; case o=>
+               //; rewrite /bnodes_triple/terms_triple
+               => id id0 id1 sib pii b; rewrite filter_undup ?undup_idem /mkPartition
+               => /= singl; try (move: singl; rewrite /undup_idem bnodes_cons /bnodes_triple /terms_triple filter_undup /= undup_bnodes).
+        (* room for improvement *)
+        + apply no_bnodes_same_partition. by rewrite /bnodes_triple filter_undup. apply (IHts b singl).
+        + apply no_bnodes_same_partition. by rewrite /bnodes_triple filter_undup. apply (IHts b singl).
+        (* =============== *)
+        + case e: (Bnode id \in bnodes {| graph := ts |})=> singl.
+        - by apply (IHts b singl).
+        - by case: singl=> _ -> /=; rewrite eq_hash_refl.
+          (* =============== *)
+          + case: (Bnode id1 \in bnodes {| graph := ts |})=> singl.
+        - by apply (IHts b singl).
+        - by case: singl=> _ -> /=; rewrite eq_hash_refl.
+          (* =============== *)
+          + case: (Bnode id1 \in bnodes {| graph := ts |})=> singl.
+        - by apply (IHts b singl).
+        - by case: singl=> _ -> /=; rewrite eq_hash_refl.
+          (* =============== *)
+          + move: singl.
+            have b_def : (bnodes_triple
+                            {|
+                              subject := Bnode id1;
+                              predicate := Iri id0;
+                              object := Bnode id;
+                              subject_in_IB := sib ;
+                              predicate_in_I := pii
+                            |}) =
+                           (if Bnode id1 \in [:: Bnode id] then [:: Bnode id] else [:: Bnode id1; Bnode id]).
+            move=> ? ?. by rewrite /bnodes_triple /terms_triple filter_undup /=.
+            rewrite bnodes_cons /bnodes_triple filter_undup -b_def -bnodes_cons => singl.
+            rewrite /= -b_def -bnodes_cons singl.
+            have isbb: is_bnode b. by apply (b_in_bnode_is_bnode singl).
+            by rewrite /= (eq_hash_refl isbb); case: b isbb singl.
+      Qed.
+
+
+    End Partition.
+
+    Section Blabel.
+      Variable hashBag : seq h -> h.
+      Hypothesis hashBag_assoc : forall (l1 l2 l3: seq h),
+          hashBag ([:: hashBag (l1 ++ l2)] ++ l3) = hashBag (l1 ++ [:: hashBag (l2 ++ l3)]).
+      Hypothesis hashBag_comm : forall (l1 l2: seq h),
+          hashBag (l1 ++ l2) = hashBag (l2 ++ l1).
+
+      Lemma hasTuple_neq_errorP s: hashTuple s = herror -> False.
+      Proof. by apply /eqP; rewrite /negb hashTuple_neq_error. Qed.
+
+
+      Section Algorithm1.
+
+        Definition new_hash (s p o : hterm) gacc h_dflt : option ((hash B) * (hash B)) :=
+          if s is Bnode hb
+          then
+            let c := hashTuple [:: (term_hash o) ; (term_hash p) ; h_dflt] in
+            let b_curr := lookup_bnode_in_graph_default gacc (input hb) in
+            Some (hb,(mkHinput (input hb) (hashBag [:: c ; b_curr ])))
+          else None.
+
+        Definition new_hash_fwd (s p o: hterm) gacc : option ((hash B) * (hash B)) :=
+          new_hash s p o gacc hfwd.
+
+        Definition new_hash_bwd (s p o : hterm) gacc : option ((hash B) * (hash B)) :=
+          new_hash o p s gacc hbwd.
+
+        (* Algorithm 1, lines 12-17
+       update the hashes of blank nodes using the neighborhood
+       it hashes differently outgoing edges from incoming ones *)
+        Definition update_bnodes (g : hgraph) : hgraph :=
+          let fix help g gacc hfun :=
+            match g with
+            | nil => gacc
+            | cons t ts => let (s,p,o,_,_) := t : htriple in
+                           let newhash := hfun s p o gacc in
+                           if newhash is Some (hb,hb')
+                           then let gacc' := replace_bnode hb hb' gacc in
+                                help ts gacc' hfun
+                           else help ts gacc hfun
+            end in
+          let g_fwd := help g g new_hash_fwd in
+          help g g_fwd new_hash_bwd.
+
+        (* Algorithm 1, lines 9-18
+       the iteration: computes the update of blank nodes until
+           - the partition is fine
+           - the partition did not change with respect to the previous one
+         *)
+        Fixpoint iterate (g : hgraph) (fuel : nat) : hgraph :=
+          match fuel with
+          | O => g
+          | S n' =>
+              let h := update_bnodes g in
+              if cmp_partition g h || is_fine (mkPartition h) then h else
+                iterate h n'
+          end.
+
+
+        Definition hashNodes_initialized (g : hgraph) : hgraph :=
+          iterate g (size (graph g)).
+
+        (* need the lemma stating hashNodes terminates without
+       getting out of fuel *)
+        (* Algorithm 1*)
+        Definition hashNodes (g : rdf_graph _ _ _) : hgraph :=
+          hashNodes_initialized (init_hash g).
+
+      End Algorithm1.
+
+      Section Algorithm2.
+        (* Definition 4.6 ≡ ~G *)
+        Definition reachability_rel (g : hgraph) (t1 t2 : htriple) : bool :=
+          let (s1, _, o1, _, _) := t1 in
+          let (s2, _, o2, _, _) := t2 in
+          let s1s2 := (s1 == s2) && is_bnode s1 in
+          let s1o2 := (s1 == o2) && is_bnode s1 in
+          let o1s2 := (o1 == s2) && is_bnode o1 in
+          let o1o2 := (o1 == o2) && is_bnode o1 in
+          s1s2 || s1o2 || o1s2 || o1o2.
+
+        (* Algorithm 2, line 2:
+       computes the connected components based on definition 4.6 (~G)
+         *)
+        Definition blank_node_split (t u v : Type) (g : rdf_graph t u v) : seq (rdf_graph t u v).
+        Proof.
+        (* compute the graph G,
+         where V := g and
+         (t,u) : (triple I B L * triple I B L) \in E iff
+         [:: t ; u] is graph and bnodes(t) ∩ bnodes(u) ≠ ϕ
+
+       Then compute the connected componens using reachability rel*)
+        Admitted.
+
+        (* The graph that contains all (and only the) ground triples of G *)
+        Definition ground_split {t u v : Type} (g : rdf_graph t u v) : rdf_graph t u v :=
+          let groundTriples := filter (fun t => is_ground_triple t) g in
+          mkRdfGraph groundTriples.
+
+        Lemma merge_split {t u v : Type} (g : rdf_graph t u v) :
+          merge_rdf_graph (merge_seq_rdf_graph (blank_node_split g)) (ground_split g) = g.
+        Admitted.
+
+        (* Algorithm 2 *)
+        Definition hashBnodesPerSplit (g : hgraph) : hgraph :=
+          let splitG := blank_node_split g in
+          foldr (@merge_rdf_graph _ _ _) (empty_rdf_graph _ _ _) splitG.
+
+      End Algorithm2.
+
+      Section Algorithm3.
+
+        (* Algorithm 3, lines 13-14 when color refine is hashBnodes_initialized.
+       b is_bnode *)
+        Definition distinguishBnode g (color_refine : hgraph -> hgraph ) (b : hash B) : hgraph :=
+          let b' := mark_hash b in
+          let g' := replace_bnode b b' g in
+          color_refine g'.
+
+
+        (* give partition and proof that partition is not fine *)
+        (* or compute it again ... *)
+        (* Algorithm 3, function distinguish, lines 9-20
+       lines 16-18 were moved to a higher level: should consume more space
+       FIXME just call distinguish_ with not fine partitions so
+       is not needed to repeat the question *)
+        Fixpoint distinguish_ g (color : hgraph -> hgraph) (fuel:nat) : hgraph :=
+          match fuel with
+          | O => g
+          | S n' =>
+              let P := mkPartition g in
+              if is_fine P then g
+              else
+                let p := choose_part P in
+                let gs := map (distinguishBnode g color) p in
+                let just_fine := (fun g: hgraph =>
+                                    if is_fine (mkPartition g) then g
+                                    else distinguish_ g color n') in
+                choose_graph (map just_fine gs)
+          end.
+
+        (* Algorithm 3, function distinguish
+       when color_refine is hashBnodes_initialized *)
+        Definition distinguish g (color_refine : hgraph -> hgraph) : hgraph :=
+          distinguish_ g color_refine (size g).
+
+      End Algorithm3.
+
+      Section Isocanonicalise.
+
+        Definition isoCanonicalTemplate g (color color_refine: hgraph -> hgraph)
+          p_refining : rdf_graph I B L:=
+          let g' := color (init_hash g) in
+          let P := mkPartition g' in
+          let g_iso := if is_fine P then g' else p_refining g' color_refine in
+          label g_iso.
+
+        (* first approach *)
+        Definition justDistinguish g :=
+          isoCanonicalTemplate g id id distinguish.
+
+        Lemma distinguish_preserves_isomorphism g : iso (justDistinguish g) g.
+        Proof.
+          rewrite /iso/justDistinguish/isoCanonicalTemplate/is_iso.
+          case (is_fine (mkPartition (init_hash g))).
+          case g=> g'. elim g'=> [|t ts ihts].
+          - exists id. split.
+            + by exists id.
+                        + by rewrite relabeling_id.
+                        -
+                          (* need to build μ. and μ bij. *)
+        Admitted.
+
+        Definition isoCanonicalNoIter g :=
+          isoCanonicalTemplate g update_bnodes update_bnodes distinguish.
+
+        Definition isoCanonicalIter g :=
+          isoCanonicalTemplate g hashNodes_initialized hashNodes_initialized distinguish.
+
+        Definition blabel g :=
+          isoCanonicalTemplate g hashBnodesPerSplit hashNodes_initialized distinguish.
+
+      End Isocanonicalise.
+    End Blabel.
+
+    Section Kmapping.
+
+      Definition k_distinguish bns : seq (term I (hash B) L) :=
+        let fix help bns n :=
+          match bns with
+          | nil => nil
+          | trm :: trms => app_n mark_bnode trm n :: help trms (S n)
+          end in
+        help bns 0.
+
+      Definition ak_mapping (g : rdf_graph I B L) : seq hterm :=
+        let bns := bnodes (init_hash g) in
+        mapi (app_n mark_bnode) bns.
+
+      Lemma empty_ak_mapping : ak_mapping (mkRdfGraph [::]) = [::]. Proof. by []. Qed.
+
+      Definition build_kmapping_from_seq (trms : seq hterm) : B -> B :=
+        fun b =>
+          if has (eqb_b_hterm b) trms then
+            let the_bnode := nth (Bnode (mkHinput b herror)) trms (find (eqb_b_hterm b) trms) in
+            to_string (lookup_hash_default the_bnode)
+          else
+            b.
+
+      Lemma inv_of_ak_mapping g : exists mu,
+          (relabeling mu g) == (relabeling (build_kmapping_from_seq (ak_mapping g)) g).
+      Proof. by exists (build_kmapping_from_seq (ak_mapping g)). Qed.
+
+      Lemma inv_of_perm_ak_mapping g (p : seq hterm) :
+        p \in (permutations (ak_mapping g)) -> (*no need for this*)
+              exists mu, (relabeling mu g) == (relabeling (build_kmapping_from_seq p) g).
+      Proof.
+        by exists (build_kmapping_from_seq p).
+      Qed.
+
+      Definition k_mapping (g : rdf_graph I B L) : rdf_graph I B L :=
+        let all_maps :=
+          map (mapi (app_n mark_bnode)) (permutations (bnodes (init_hash g))) in
+        let mus := map build_kmapping_from_seq all_maps in
+        let isocans := map (fun mu => relabeling mu g) mus in
+        foldl Order.max (mkRdfGraph [::]) isocans.
+
+      Lemma k_mapping_seq_uniq_graph g: uniq (mapi (app_n mark_bnode) (bnodes (init_hash g))).
+      Proof.
+        rewrite /mapi; pose g' := init_hash g.
+        rewrite map_inj_in_uniq; first by apply (zip_uniq_l _ (uniq_bnodes g')).
+        move=> [t n] [u m] /in_zip/andP [tin_bns n_iota] /in_zip/andP [uin_bns m_iota] /= eq_app_n.
+        case: t tin_bns uin_bns eq_app_n; case: u
+            => nt nu; rewrite ?i_in_bnodes ?l_in_bnodes // => nu_bns nt_bns injH.
+        by apply /eqP; rewrite xpair_eqE; apply (can_app_n_mb_init nu_bns nt_bns injH).
+      Qed.
+
+      Lemma k_mapping_seq_uniq_perm_eq g s: perm_eq s (bnodes (init_hash g)) -> uniq (mapi (app_n mark_bnode) s).
+      Proof. rewrite /mapi perm_sym=> perm_eq. rewrite map_inj_in_uniq. apply uniq_zip_iota.
+             move=> [x1 n] [y1 m] /in_zip/andP [x1_ins n_iniota] /in_zip/andP [y1_ins m_iniota] /=.
+             have : is_bnode x1. apply (in_all x1_ins); rewrite -(perm_all _ perm_eq); apply all_bnodes.
+             have : is_bnode y1. apply (in_all y1_ins); rewrite -(perm_all _ perm_eq); apply all_bnodes.
+             case :y1 x1_ins y1_ins; case x1=> // namey namex y_ins x_ins _ _.
+             have y1_init: Bnode namey \in (bnodes (init_hash g)). rewrite (perm_mem perm_eq). apply y_ins.
+             have x1_init: Bnode namex \in (bnodes (init_hash g)). rewrite (perm_mem perm_eq). apply x_ins.
+             by move=> ?; apply /eqP; rewrite xpair_eqE; apply (can_app_n_mb_init y1_init).
+      Qed.
+
+      Lemma injection_kmap b b' ht s (eb: eqb_b_hterm b ht) (eb': eqb_b_hterm b' ht):
+        (build_kmapping_from_seq (mapi (app_n mark_bnode) s) b) =
+          (build_kmapping_from_seq (mapi (app_n mark_bnode) s) b').
+      Proof. suffices : b = b'. by move=> ->.
+             by apply (eqb_b_hterm_trans eb eb'). Qed.
+
+      Lemma map_kmap b n s :
+        (build_kmapping_from_seq s b) = n ->
+        (has (eqb_b_hterm b) s) ->
+        forall s' (f : B -> B), injective f -> s' = map (relabeling_hterm f) s ->
+                                (build_kmapping_from_seq s' (f b)) = n.
+      Proof.
+        elim: s=> [| hd tl IHtl]; first by rewrite has_nil.
+        move=> beq has_b s'; case: s'=> [//| hd' tl'] f injF [eqhd eqtl].
+        move: IHtl; rewrite /build_kmapping_from_seq eqhd eqtl -map_cons -has_map; last by apply injF.
+        rewrite has_b /= -eqb_b_hterm_relabel; last by apply injF. rewrite /= in has_b.
+        case/orP: has_b beq; first by rewrite /build_kmapping_from_seq=> H /=; rewrite H; case hd=> // name /=.
+        + rewrite /build_kmapping_from_seq /= ; case e: (eqb_b_hterm b hd)
+                  => /=; first by move=> _; rewrite -lookup_hash_relabeling.
+          move=> /= has_tl /=; rewrite has_tl=> eq IHtl.
+          have IHtl' := IHtl eq isT tl' f injF eqtl.
+          by rewrite eqtl -has_map ?has_tl in IHtl'; last by apply injF.
+      Qed.
+
+      Lemma all_kmaps_bijective g : List.Forall (fun mu => bijective mu) [seq build_kmapping_from_seq i
+                                                                         | i <- [seq mapi (app_n mark_bnode) i
+                                                                                | i <- permutations (bnodes (init_hash g))]].
+      Proof.
+        have map2Listmap U V (f : U -> V) (s : seq U) : map f s = List.map f s. admit.
+        have nth2Listnth U (d : U) (s : seq U) n : nth d s n = List.nth n s d. admit.
+        have size2Listlength U (s : seq U) : List.length s = size s. admit.
+        rewrite !map2Listmap !List.Forall_map.
+        suffices step s : perm_eq s (bnodes (init_hash g)) -> bijective (build_kmapping_from_seq (mapi (app_n mark_bnode) s)).
+        apply/List.Forall_nth=> i d lti. apply: step. rewrite -mem_permutations -nth2Listnth. apply: mem_nth.
+        by rewrite -size2Listlength; apply/ltP.
+        (* by using k_mapping_seq_uniq_perm_eq *)
+        admit.
+      Admitted.
+
+      (* TODO *)
+      (* only way of k_mapping g = [::] -> g = [::]*)
+      Lemma inv_of_k_mapping g : exists mu, (relabeling mu g) == (k_mapping g) /\ bijective mu.
+      Proof.
+        (* FIX ME*)
+        (* have step1 : k_mapping g = mkRdfGraph [::] \/ *)
+        (*                (k_mapping g) \in [seq relabeling mu0 g *)
+        (*                                  | mu0 <- [seq build_kmapping_from_seq i *)
+        (*                                           | i <- [seq mapi (app_n mark_bnode) i *)
+        (*                                                  | i <- permutations *)
+        (*                                                           (bnodes (init_hash g))]]]. *)
+        (* rewrite /=. /k_mapping relabeling_id; apply: foldl_op. *)
+        (* case: step1=> [ -> | in_tail ]. *)
+        (* + exists id; split. *)
+        (* - by rewrite relabeling_id. *)
+        (* - exact: id_bij.  *)
+        (*   + have [mu eq_mu_map] : exists mu : B -> B, relabeling mu g == k_mapping g. *)
+        (*     exact: relabeling_mu_inv in_tail. *)
+        (*     exists mu. split; first exact eq_mu_map. *)
+        (*     (* needs mu to have eqType, could be a finfun *) *)
+        (*     have fin_mu : (seq_sub (bnodes g)) -> B. *)
+        (*     Fail move: (finfun (fun b => b)). *)
+        (*     admit. *)
+        (* Fail fin_mu \in in_tail. *)
+      Admitted.
+
+      (* TODO *)
+      (* USES inv_of_k_mapping *)
+      Lemma k_mapping_iso_output : mapping_is_iso k_mapping.
+      Proof. move=> g; case (inv_of_k_mapping g)=> μ [rel_eq_kmap bijmu].
+             exists μ. split. exact: bijmu. by rewrite eq_sym.
+      Qed.
+
+      Lemma k_mapping_dont_manipulate_names : (dt_names k_mapping).
+      Proof.
+        rewrite /dt_names=> g μ bijmu.
+        case g=> g'; rewrite /k_mapping.
+        suffices ->:
+          [seq relabeling mu {| graph := g' |}
+          | mu <- [seq build_kmapping_from_seq i
+                  | i <- [seq mapi (app_n mark_bnode) i
+                         | i <- permutations (bnodes (init_hash {| graph := g' |}))]]] =
+                   [seq relabeling mu (relabeling μ {| graph := g' |})
+                   | mu <- [seq build_kmapping_from_seq i
+                           | i <- [seq mapi (app_n mark_bnode) i
+                                  | i <- permutations (bnodes (init_hash (relabeling μ {| graph := g' |})))]]].
+        by [].
+        elim e: [seq build_kmapping_from_seq i
                 | i <- [seq mapi (app_n mark_bnode) i
-                       | i <- permutations (bnodes (init_hash {| graph := g' |}))]]] =
-                 [seq relabeling mu (relabeling μ {| graph := g' |})
-                 | mu <- [seq build_mapping_from_seq i
-                         | i <- [seq mapi (app_n mark_bnode) i
-                                | i <- permutations (bnodes (init_hash (relabeling μ {| graph := g' |})))]]].
-      by [].
-      elim e: [seq build_mapping_from_seq i
-              | i <- [seq mapi (app_n mark_bnode) i
-                     | i <- permutations (bnodes (init_hash {| graph := g' |}))]]=> [|mu' mus IHmu].
-      have ->: [seq build_mapping_from_seq i
-               | i <- [seq mapi (app_n mark_bnode) i
-                      | i <- permutations (bnodes (init_hash (relabeling μ {| graph := g' |})))]] = [::].
-      admit.
-      by [].
-      case e2: [seq build_mapping_from_seq i
-               | i <- [seq mapi (app_n mark_bnode) i
-                      | i <- permutations (bnodes (init_hash (relabeling μ {| graph := g' |})))]]=> [|mu'' mus'].
-      admit. (* this is a contradiction *)
-      rewrite /= relabeling_comp.
-      f_equal.
-      have mu_ext: mu' =1 (mu'' \o μ).
-      (* using map_kmap *)
-      admit.
-      by rewrite (relabeling_ext {| graph := g' |} mu_ext).
-      (* this should be exactically IHmu *)
-      admit.
-    Admitted.
+                       | i <- permutations (bnodes (init_hash {| graph := g' |}))]]=> [|mu' mus IHmu].
+        have ->: [seq build_kmapping_from_seq i
+                 | i <- [seq mapi (app_n mark_bnode) i
+                        | i <- permutations (bnodes (init_hash (relabeling μ {| graph := g' |})))]] = [::].
+        admit.
+        by [].
+        case e2: [seq build_kmapping_from_seq i
+                 | i <- [seq mapi (app_n mark_bnode) i
+                        | i <- permutations (bnodes (init_hash (relabeling μ {| graph := g' |})))]]=> [|mu'' mus'].
+        admit. (* this is a contradiction *)
+        rewrite /= relabeling_comp.
+        f_equal.
+        have mu_ext: mu' =1 (mu'' \o μ).
+        (* using map_kmap *)
+        admit.
+        by rewrite (relabeling_ext {| graph := g' |} mu_ext).
+        (* this should be exactically IHmu *)
+        admit.
+      Admitted.
 
-    (* USES inv_of_k_mapping *)
-    Lemma k_mapping_isocan : isocanonical_mapping k_mapping.
-    Proof. by apply: isocanonical_mapping_dt_out k_mapping_iso_output k_mapping_dont_manipulate_names. Qed.
+      (* USES inv_of_k_mapping *)
+      Lemma k_mapping_isocan : isocanonical_mapping k_mapping.
+      Proof. by apply: isocanonical_mapping_dt_out k_mapping_iso_output k_mapping_dont_manipulate_names. Qed.
 
-    Lemma relabeling_mu_inv_bij (g : rdf_graph I B L) (fs : seq (B -> B)) :
-      List.Forall (fun mu => bijective mu) fs ->
-      exists (mu : B->B), relabeling mu g == k_mapping g /\ bijective mu.
-    Proof. move => all_bij.
-           apply inv_of_k_mapping.
-    Qed.
+      Lemma relabeling_mu_inv_bij (g : rdf_graph I B L) (fs : seq (B -> B)) :
+        List.Forall (fun mu => bijective mu) fs ->
+        exists (mu : B->B), relabeling mu g == k_mapping g /\ bijective mu.
+      Proof. move => all_bij.
+             apply inv_of_k_mapping.
+      Qed.
 
-    Lemma k_mapping_iso g : iso (k_mapping g) g.
-    Proof. rewrite /iso/is_iso.
-           have H:exists mu : B -> B, relabeling mu g == k_mapping g /\ bijective mu. apply inv_of_k_mapping.
-           move: H=> [mu [eq bij]].
-           exists mu; split; first by exact: bij.
-           by rewrite eq_sym; apply eq.
-    Qed.
+      Lemma k_mapping_iso g : iso (k_mapping g) g.
+      Proof. rewrite /iso/is_iso.
+             have H:exists mu : B -> B, relabeling mu g == k_mapping g /\ bijective mu. apply inv_of_k_mapping.
+             move: H=> [mu [eq bij]].
+             exists mu; split; first by exact: bij.
+             by rewrite eq_sym; apply eq.
+      Qed.
+
+    End Kmapping.
 
   End IsoCanAlgorithm.
 
